src/Refinement_AlgorithmicPF_Algorithmic.v
@@ -1,0 +1,45 @@
+Require Import Relations.
+Require Import EquivDec.
+Require Import Equality.
+Require Import List.
+Require Import Bool.
+Require Import Lia.
+Require Import NArith.
+Require Import PArith.
+Require Import ZArith.
+Require Import FMapPositive.
+Require Import FSetPositive.
+Require Import EquivDec.
+Require Import sflib.
+
+Require Import Basic.
+Require Import Order.
+Require Import Time.
+Require Import Lang.
+Require Import Promising.
+Require Import Algorithmic.
+
+Set Implicit Arguments.
+
+
+Lemma rtc_state_step_certify_inv
+      m1 m2 tid st lc l
+      (STEPS: rtc (Machine.step ExecUnit.state_step) m1 m2)
+      (NOPROMISE: Machine.no_promise m2)
+      (FIND: IdMap.find tid m1.(Machine.tpool) = Some (st, lc))
+      (CERTIFY: certify tid (ExecUnit.mk st lc m1.(Machine.mem)) l):
+  l = bot.
+Proof.
+Admitted.
+
+Theorem algorithmic_pf_to_algorithmic
+        p m
+        (EXEC: AMachine.pf_exec p m):
+  AMachine.exec p m.
+Proof.
+  inv EXEC. econs; cycle 1; ss.
+  { instantiate (1 := AMachine.mk m (IdMap.map (fun _ => bot) p)). ss. }
+  etrans.
+  { eapply AMachine.rtc_step_mon; cycle 1; eauto. right. ss. }
+  admit. (* use rtc_state_step_certify_inv *)
+Admitted.
