src/Refinement_PromisingPF_AlgorithmicPF.v
@@ -1,0 +1,57 @@
+Require Import Relations.
+Require Import EquivDec.
+Require Import Equality.
+Require Import List.
+Require Import Bool.
+Require Import Lia.
+Require Import NArith.
+Require Import PArith.
+Require Import ZArith.
+Require Import FMapPositive.
+Require Import FSetPositive.
+Require Import EquivDec.
+Require Import sflib.
+
+Require Import Basic.
+Require Import Order.
+Require Import Time.
+Require Import Lang.
+Require Import Promising.
+Require Import Algorithmic.
+
+Set Implicit Arguments.
+
+
+Lemma rtc_state_step_certify_bot
+      m1 m2 tid st lc
+      (STEPS: rtc (Machine.step ExecUnit.state_step) m1 m2)
+      (NOPROMISE: Machine.no_promise m2)
+      (FIND: IdMap.find tid m1.(Machine.tpool) = Some (st, lc)):
+  certify tid (ExecUnit.mk st lc m1.(Machine.mem)) bot.
+Proof.
+  revert tid st lc FIND NOPROMISE. induction STEPS.
+  { econs; eauto; ss.
+    - eapply NOPROMISE. eauto.
+    - funext. unfold bot, fun_bot. i. propext. econs; ss. i. inv H.
+      + inv LOCKS. ss.
+      + inv LOCKS. ss.
+  }
+  i. inv H. exploit IHSTEPS; ss.
+  { rewrite TPOOL, IdMap.add_spec, FIND.
+    instantiate (1 := if equiv_dec tid tid0 then lc2 else lc).
+    instantiate (1 := if equiv_dec tid tid0 then st2 else st).
+    condtac; ss.
+  }
+  condtac.
+  - inversion e. subst. rewrite FIND in FIND0. inv FIND0.
+    admit. (* certify is preserved if I executed a state_step. *)
+  - admit. (* certify is preserved if another thread is executed. *)
+Admitted.
+
+Theorem promising_pf_to_algorithmic_pf
+        p m
+        (EXEC: Machine.pf_exec p m):
+  AMachine.pf_exec p m.
+Proof.
+  inv EXEC. exploit rtc_state_step_certify_bot; eauto.
+Admitted.
