src/Refinement_PromisingPF_Promising.v
@@ -1,0 +1,33 @@
+Require Import Relations.
+Require Import EquivDec.
+Require Import Equality.
+Require Import List.
+Require Import Bool.
+Require Import Lia.
+Require Import NArith.
+Require Import PArith.
+Require Import ZArith.
+Require Import FMapPositive.
+Require Import FSetPositive.
+Require Import EquivDec.
+Require Import sflib.
+
+Require Import Basic.
+Require Import Order.
+Require Import Time.
+Require Import Lang.
+Require Import Promising.
+
+Set Implicit Arguments.
+
+
+Theorem promising_pf_to_promising
+        p m
+        (EXEC: Machine.pf_exec p m):
+  Machine.exec p m.
+Proof.
+  inv EXEC. econs; eauto.
+  etrans.
+  - eapply Machine.rtc_step_mon; cycle 1; eauto. right. ss.
+  - eapply Machine.rtc_step_mon; cycle 1; eauto. left. ss.
+Qed.
